\documentclass{article}
\usepackage[utf8]{inputenc}
\usepackage{relsize}
\usepackage{geometry}
\usepackage{tikz}
\usetikzlibrary{automata, positioning, arrows}
\tikzset{node distance=2.5cm, % Minimum distance between two nodes. Change if necessary.
every state/.style={ % Sets the properties for each state
semithick,
fill=gray!10},
initial text={}, % No label on start arrow
double distance=2pt, % Adjust appearance of accept states
every edge/.style={ % Sets the properties for each transition
draw,->,>=stealth', % Makes edges directed with bold arrowheads
auto,semithick}}



\geometry{
 a4paper,
 total={170mm,257mm},
 left=20mm,
 top=20mm,
}

\title{Homework 1\\[0.2em]\smaller{}CSC 445-01: Theory of Computation}
\author{Matthew Mabrey, Luke Kurlandski}
\date{\today}

\begin{document}

\maketitle

\section*{Question I}

\section*{Question II}

\subsection*{a}

\subsection*{b}

\subsection*{c}

\section*{Question III}
We will prove
$$
P(n) \colon \sum^n_{i=1} \frac{1}{i(i+1)} = \frac{n}{n+1} \;\; \biggr | \;\; n \geq 0, n \in Z
$$
Base case:
\begin{eqnarray*}
P(0) &\colon& \sum^n_{i=1} \frac{1}{i(i+1)} = \frac{n}{n+1} \\
&\colon& \sum^0_{i=1} \frac{1}{i(i+1)} = \frac{0}{0+1} \\
&\colon& 0 = 0 \\
&\colon& \textrm{TRUE}
\end{eqnarray*}
Inductive Hypothesis:
$$
P(k) \colon \sum^k_{i=1} \frac{1}{i(i+1)} = \frac{k}{k+1} \;\; \biggr | \;\; k \geq 0, k \in Z
$$
Induction:
\begin{eqnarray*}
P(k+1) \colon \;\; \frac{k+1}{k+2} &=& \sum^{k+1}_{i=1} \frac{1}{i(i+1)}  \\
&=& \sum^k_{i=1} \frac{1}{i(i+1)} + \frac{1}{(k+1)((k+1)+1)} \\
&=& \frac{k}{k+1} + \frac{1}{(k+1)(k+2)} \\ 
&=& \frac{k(k+2) + 1}{(k+1)(k+2)} \\ 
&=& \frac{(k+1)^2}{(k+1)(k+2)} \\
\frac{k+1}{(k+2)} &=& \frac{k+1}{(k+2)} \\
P(k+1) \colon \textrm{TRUE}
\end{eqnarray*}
Conclusion:
$$
\left (  P(0) \; \land \; \biggr ( P(k) \rightarrow P(k+1) \biggr ) \right ) \rightarrow P(n) 
$$

\section*{Question IV}

\subsection*{Truth Table}
\begin{displaymath}
\begin{array}{c c|c|c|c|c|c} % bars control columns
p & q & 
(p \rightarrow q) \land (p \rightarrow \neg q) & 
p \land (p \rightarrow q) & 
(p \rightarrow q) \land (\neg p \rightarrow q) &
p \iff (p \iff q) &
q \land (p \rightarrow q)
\\ 
\hline
T & T & F & T & T & T & T \\
T & F & F & F & F & F & F \\
F & T & T & F & T & F & T \\
F & F & T & F & F & F & F 
\end{array}
\end{displaymath}

\subsection*{Equivalence}
\begin{displaymath}
\begin{array}{c|c|c} % bars control columns
Problem & Original & Simplified \\
\hline
a & (p \rightarrow q) \land (p \rightarrow \neg q) & \neg p \\ 
b & p \land (p \rightarrow q) & p \land q \\
c & (p \rightarrow q) \land (\neg p \rightarrow q) & q \\
d & p \iff (p \iff q) & p \land q \\
e & q \land (p \rightarrow q) & q
\end{array}
\end{displaymath}

\section*{Question V}

\[ \textrm{Given } P = \theta, Q=\{\epsilon\}, R=\{aba, bcb, cac\}, \textrm{ and } S=\{aba, abc, abb\}\]

\subsection{1}
\textit{P $\subset$ Q} is correct because $\theta$ is a proper subset all of sets (besides itself) since all elements contained in P are contained within Q, while P $\neq$ Q.

\subsection{2}
\textit{R $\cap$ S} = \{\textit{aba}\} because $\cap$ is the intersection of both sets and the only element both sets share is \textit{aba}.

\subsection{3}
\textit{R $\triangle$ S} = \{\textit{bcb, cac, abc, abb}\} because $\triangle$ is the disjoint union of both sets. In other words, the set of elements from both sets that are not shared between them. Thus the resulting set is every element besides the shared element \textit{aba} from the previous problem.

\subsection{4}
\textit{$\vert\vert$R $\vert\vert$} = 3 because the cardinality of a set is the number of elements contained within within the set.

\section*{Question VI}

\[ \textrm{Given } P = (x \rightarrow y) \land (y \rightarrow z) \textrm{ where x, y, and z are boolean variables}\]

\subsection{1} 
The value of \textit{P} is false when \textit{x, z = true} and \textit{y = false} because the first implication \textit{(x $\rightarrow$ y)} in the \textit{AND} statement evaluates to false. This is because the hypothesis in the implication is true while the conclusion is false, which is the only case where the implication will evaluate to false.

\subsection{2} 
The value of \textit{P} is again false when \textit{y = true} and \textit{x, z = false} because the second implication \textit{(y $\rightarrow$ z)} in the \textit{AND} statement evaluates to false. The same reasoning as above applies where the hypothesis in the implication is true, while the conclusion is false, causing the implication to be false.

\section*{Question VII}

\subsection{1} 

Let the 4-state finite automaton that accepts the words over \{\textit{a}, \textit{b}\} that end with \textit{aba} be formally defined by

\[
M = \left(\{q_0, q_1, q_2, q_3\}, \{\textit{a},
\textit{b}\}, \delta, q_0, \{q_3\} \right),
\]
\[\textrm{where } \delta \textrm{ is given by} \] 
\begin{center}
    \begin{tabular}{c|cc}
    & \textit{a} & \textit{b}\\ \hline
    $q_0$ & $q_1$ & $q_0$ \\
    $q_1$ & $q_1$ & $q_2$ \\
    $q_2$ & $q_3$ & $q_0$ \\
    $q_3$ & $q_1$ & $q_2$
    \end{tabular}
\end{center}

The state diagram then constructed from this definition is thus

\begin{center}
    \begin{tikzpicture}
    \node[state, initial] (q0) {$q_0$};
    \node[state, right of=q0] (q1) {$q_1$};
    \node[state, right of=q1] (q2) {$q_2$};
    \node[state, accepting, right of=q2] (q3) {$q_3$};
    \draw (q0) edge node {\tt a} (q1);
    \draw (q0) edge[loop below] node {\tt b} (q0);
    \draw (q1) edge[loop below] node {\tt a} (q1);
    \draw (q1) edge node {\tt b} (q2);
    \draw (q2) edge node {\tt a} (q3);
    \draw (q2) edge[above, bend right] node {\tt b} (q0);
    \draw (q3) edge[below, bend left] node {\tt a} (q1);
    \draw (q3) edge[above, bend right] node {\tt b} (q2);
    \end{tikzpicture}
\end{center}

\subsection{2}

Let the 6-state finite automaton that accepts the words over \{0, 1\} that contain either 000 or 111 be formally defined by

\[
M = \left(\{q_0, q_1, q_2, q_3, q_4, q_5\}, \{0,
1\}, \delta, q_0, \{q_5\} \right),
\]
\[\textrm{where } \delta \textrm{ is given by} \] 
\begin{center}
    \begin{tabular}{c|cc}
    & \textit{a} & \textit{b}\\ \hline
    $q_0$ & $q_1$ & $q_0$ \\
    $q_1$ & $q_1$ & $q_2$ \\
    $q_2$ & $q_3$ & $q_0$ \\
    $q_3$ & $q_1$ & $q_2$ \\
    $q_4$ & $q_1$ & $q_2$ \\
    $q_5$ & $q_1$ & $q_2$
    \end{tabular}
\end{center}

The state diagram then constructed from this definition is thus

\begin{center}
    \begin{tikzpicture}
    \node[state, initial] (q0) {$q_0$};
    \node[state, right of=q0, above of=q0] (q1) {$q_1$};
    \node[state, right of=q1, below of=q0] (q2) {$q_2$};
    \node[state, right of=q1] (q3) {$q_3$};
    \node[state, right of=q2] (q4) {$q_4$};
    \node[state, right of=q3, below of=q3, accepting] (q5) {$q_5$};
    \draw (q0) edge node {\tt 0} (q1);
    \draw (q0) edge node {\tt 1} (q2);
    \draw (q1) edge node {\tt 0} (q3);
    \draw (q1) edge[left, bend right=10] node {\tt 1} (q2);
    \draw (q2) edge[right, bend right=10] node {\tt 0} (q1);
    \draw (q2) edge node {\tt 1} (q4);
    \draw (q3) edge node {\tt 0} (q5);
    \draw (q3) edge[near start] node {\tt 1} (q2);
    \draw (q4) edge[right, near start] node {\tt 0} (q1);
    \draw (q4) edge node {\tt 1} (q5);
    \draw (q5) edge[loop above] node {\tt 0} (q5);
    \draw (q5) edge[loop below] node {\tt 1} (q5);
    
    \end{tikzpicture}
\end{center}

\end{document}
